dropped "run" marker in monad syntax

src/HOL/Library/State_Monad.thy
@@ -56,39 +56,29 @@ text {*
   we use a set of monad combinators:
 *}
 
-notation fcomp (infixl ">>" 60)
-notation (xsymbols) fcomp (infixl "\<guillemotright>" 60)
-notation scomp (infixl ">>=" 60)
-notation (xsymbols) scomp (infixl "\<guillemotright>=" 60)
+notation fcomp (infixl "o>" 60)
+notation (xsymbols) fcomp (infixl "o>" 60)
+notation scomp (infixl "o->" 60)
+notation (xsymbols) scomp (infixl "o\<rightarrow>" 60)
 
 abbreviation (input)
   "return \<equiv> Pair"
 
-definition
-  run :: "('a \<Rightarrow> 'b) \<Rightarrow> 'a \<Rightarrow> 'b" where
-  "run f = f"
-
-print_ast_translation {*
-  [(@{const_syntax "run"}, fn (f::ts) => Syntax.mk_appl f ts)]
-*}
-
 text {*
   Given two transformations @{term f} and @{term g}, they
-  may be directly composed using the @{term "op \<guillemotright>"} combinator,
-  forming a forward composition: @{prop "(f \<guillemotright> g) s = f (g s)"}.
+  may be directly composed using the @{term "op o>"} combinator,
+  forming a forward composition: @{prop "(f o> g) s = f (g s)"}.
 
   After any yielding transformation, we bind the side result
   immediately using a lambda abstraction.  This 
-  is the purpose of the @{term "op \<guillemotright>="} combinator:
-  @{prop "(f \<guillemotright>= (\<lambda>x. g)) s = (let (x, s') = f s in g s')"}.
+  is the purpose of the @{term "op o\<rightarrow>"} combinator:
+  @{prop "(f o\<rightarrow> (\<lambda>x. g)) s = (let (x, s') = f s in g s')"}.
 
   For queries, the existing @{term "Let"} is appropriate.
 
   Naturally, a computation may yield a side result by pairing
   it to the state from the left;  we introduce the
   suggestive abbreviation @{term return} for this purpose.
-
-  The @{const run} ist just a marker.
 
   The most crucial distinction to Haskell is that we do
   not need to introduce distinguished type constructors
@@ -107,22 +97,6 @@ text {*
 *}
 
 
-subsection {* Obsolete runs *}
-
-text {*
-  @{term run} is just a doodle and should not occur nested:
-*}
-
-lemma run_simp [simp]:
-  "\<And>f. run (run f) = run f"
-  "\<And>f g. run f \<guillemotright>= g = f \<guillemotright>= g"
-  "\<And>f g. run f \<guillemotright> g = f \<guillemotright> g"
-  "\<And>f g. f \<guillemotright>= (\<lambda>x. run g) = f \<guillemotright>= (\<lambda>x. g)"
-  "\<And>f g. f \<guillemotright> run g = f \<guillemotright> g"
-  "\<And>f. f = run f \<longleftrightarrow> True"
-  "\<And>f. run f = f \<longleftrightarrow> True"
-  unfolding run_def by rule+
-
 subsection {* Monad laws *}
 
 text {*
@@ -130,66 +104,14 @@ text {*
   as normalization rules for monadic expressions:
 *}
 
-lemma
-  return_scomp [simp]: "return x \<guillemotright>= f = f x"
-  unfolding scomp_def by (simp add: expand_fun_eq)
-
-lemma
-  scomp_return [simp]: "x \<guillemotright>= return = x"
-  unfolding scomp_def by (simp add: expand_fun_eq split_Pair)
-
-lemma
-  id_fcomp [simp]: "id \<guillemotright> f = f"
-  unfolding fcomp_def by simp
-
-lemma
-  fcomp_id [simp]: "f \<guillemotright> id = f"
-  unfolding fcomp_def by simp
-
-lemma
-  scomp_scomp [simp]: "(f \<guillemotright>= g) \<guillemotright>= h = f \<guillemotright>= (\<lambda>x. g x \<guillemotright>= h)"
-  unfolding scomp_def by (simp add: split_def expand_fun_eq)
-
-lemma
-  scomp_fcomp [simp]: "(f \<guillemotright>= g) \<guillemotright> h = f \<guillemotright>= (\<lambda>x. g x \<guillemotright> h)"
-  unfolding scomp_def fcomp_def by (simp add: split_def expand_fun_eq)
-
-lemma
-  fcomp_scomp [simp]: "(f \<guillemotright> g) \<guillemotright>= h = f \<guillemotright> (g \<guillemotright>= h)"
-  unfolding scomp_def fcomp_def by (simp add: split_def expand_fun_eq)
-
-lemma
-  fcomp_fcomp [simp]: "(f \<guillemotright> g) \<guillemotright> h = f \<guillemotright> (g \<guillemotright> h)"
-  unfolding fcomp_def o_assoc ..
-
-lemmas monad_simp = run_simp return_scomp scomp_return id_fcomp fcomp_id
-  scomp_scomp scomp_fcomp fcomp_scomp fcomp_fcomp
+lemmas monad_simp = Pair_scomp scomp_Pair id_fcomp fcomp_id
+  scomp_scomp scomp_fcomp fcomp_scomp fcomp_assoc
 
 text {*
   Evaluation of monadic expressions by force:
 *}
 
-lemmas monad_collapse = monad_simp o_apply o_assoc split_Pair split_comp
-  scomp_def fcomp_def run_def
-
-subsection {* ML abstract operations *}
-
-ML {*
-structure StateMonad =
-struct
-
-fun liftT T sT = sT --> HOLogic.mk_prodT (T, sT);
-fun liftT' sT = sT --> sT;
-
-fun return T sT x = Const (@{const_name return}, T --> liftT T sT) $ x;
-
-fun scomp T1 T2 sT f g = Const (@{const_name scomp},
-  liftT T1 sT --> (T1 --> liftT T2 sT) --> liftT T2 sT) $ f $ g;
-
-fun run T sT f = Const (@{const_name run}, liftT' (liftT T sT)) $ f;
-
-end;
-*}
+lemmas monad_collapse = monad_simp fcomp_apply scomp_apply split_beta
 
 
 subsection {* Syntax *}
@@ -211,7 +133,7 @@ syntax
     ("_;// _" [13, 12] 12)
   "_let" :: "pttrn \<Rightarrow> 'a \<Rightarrow> do_expr \<Rightarrow> do_expr"
     ("let _ = _;// _" [1000, 13, 12] 12)
-  "_nil" :: "'a \<Rightarrow> do_expr"
+  "_done" :: "'a \<Rightarrow> do_expr"
     ("_" [12] 12)
 
 syntax (xsymbols)
@@ -219,94 +141,54 @@ syntax (xsymbols)
     ("_ \<leftarrow> _;// _" [1000, 13, 12] 12)
 
 translations
-  "_do f" => "CONST run f"
-  "_scomp x f g" => "f \<guillemotright>= (\<lambda>x. g)"
-  "_fcomp f g" => "f \<guillemotright> g"
+  "_do f" => "f"
+  "_scomp x f g" => "f o\<rightarrow> (\<lambda>x. g)"
+  "_fcomp f g" => "f o> g"
   "_let x t f" => "CONST Let t (\<lambda>x. f)"
-  "_nil f" => "f"
+  "_done f" => "f"
 
 print_translation {*
 let
   fun dest_abs_eta (Abs (abs as (_, ty, _))) =
         let
           val (v, t) = Syntax.variant_abs abs;
-        in ((v, ty), t) end
+        in (Free (v, ty), t) end
     | dest_abs_eta t =
         let
           val (v, t) = Syntax.variant_abs ("", dummyT, t $ Bound 0);
-        in ((v, dummyT), t) end
+        in (Free (v, dummyT), t) end;
   fun unfold_monad (Const (@{const_syntax scomp}, _) $ f $ g) =
         let
-          val ((v, ty), g') = dest_abs_eta g;
-        in Const ("_scomp", dummyT) $ Free (v, ty) $ f $ unfold_monad g' end
+          val (v, g') = dest_abs_eta g;
+        in Const ("_scomp", dummyT) $ v $ f $ unfold_monad g' end
     | unfold_monad (Const (@{const_syntax fcomp}, _) $ f $ g) =
         Const ("_fcomp", dummyT) $ f $ unfold_monad g
     | unfold_monad (Const (@{const_syntax Let}, _) $ f $ g) =
         let
-          val ((v, ty), g') = dest_abs_eta g;
-        in Const ("_let", dummyT) $ Free (v, ty) $ f $ unfold_monad g' end
+          val (v, g') = dest_abs_eta g;
+        in Const ("_let", dummyT) $ v $ f $ unfold_monad g' end
     | unfold_monad (Const (@{const_syntax Pair}, _) $ f) =
         Const ("return", dummyT) $ f
     | unfold_monad f = f;
-  fun tr' (f::ts) =
-    list_comb (Const ("_do", dummyT) $ unfold_monad f, ts)
-in [(@{const_syntax "run"}, tr')] end;
+  fun contains_scomp (Const (@{const_syntax scomp}, _) $ _ $ _) = true
+    | contains_scomp (Const (@{const_syntax fcomp}, _) $ _ $ t) =
+        contains_scomp t
+    | contains_scomp (Const (@{const_syntax Let}, _) $ _ $ Abs (_, _, t)) =
+        contains_scomp t;
+  fun scomp_monad_tr' (f::g::ts) = list_comb
+    (Const ("_do", dummyT) $ unfold_monad (Const (@{const_syntax scomp}, dummyT) $ f $ g), ts);
+  fun fcomp_monad_tr' (f::g::ts) = if contains_scomp g then list_comb
+      (Const ("_do", dummyT) $ unfold_monad (Const (@{const_syntax fcomp}, dummyT) $ f $ g), ts)
+    else raise Match;
+  fun Let_monad_tr' (f :: (g as Abs (_, _, g')) :: ts) = if contains_scomp g' then list_comb
+      (Const ("_do", dummyT) $ unfold_monad (Const (@{const_syntax Let}, dummyT) $ f $ g), ts)
+    else raise Match;
+in [
+  (@{const_syntax scomp}, scomp_monad_tr'),
+  (@{const_syntax fcomp}, fcomp_monad_tr'),
+  (@{const_syntax Let}, Let_monad_tr')
+] end;
 *}
-
-
-subsection {* Combinators *}
-
-definition
-  lift :: "('a \<Rightarrow> 'b) \<Rightarrow> 'a \<Rightarrow> 'c \<Rightarrow> 'b \<times> 'c" where
-  "lift f x = return (f x)"
-
-primrec
-  list :: "('a \<Rightarrow> 'b \<Rightarrow> 'b) \<Rightarrow> 'a list \<Rightarrow> 'b \<Rightarrow> 'b" where
-  "list f [] = id"
-| "list f (x#xs) = (do f x; list f xs done)"
-
-primrec
-  list_yield :: "('a \<Rightarrow> 'b \<Rightarrow> 'c \<times> 'b) \<Rightarrow> 'a list \<Rightarrow> 'b \<Rightarrow> 'c list \<times> 'b" where
-  "list_yield f [] = return []"
-| "list_yield f (x#xs) = (do y \<leftarrow> f x; ys \<leftarrow> list_yield f xs; return (y#ys) done)"
-
-definition
-  collapse :: "('a \<Rightarrow> ('a \<Rightarrow> 'b \<times> 'a) \<times> 'a) \<Rightarrow> 'a \<Rightarrow> 'b \<times> 'a" where
-  "collapse f = (do g \<leftarrow> f; g done)"
-
-text {* combinator properties *}
-
-lemma list_append [simp]:
-  "list f (xs @ ys) = list f xs \<guillemotright> list f ys"
-  by (induct xs) (simp_all del: id_apply)
-
-lemma list_cong [fundef_cong, recdef_cong]:
-  "\<lbrakk> \<And>x. x \<in> set xs \<Longrightarrow> f x = g x; xs = ys \<rbrakk>
-    \<Longrightarrow> list f xs = list g ys"
-proof (induct xs arbitrary: ys)
-  case Nil then show ?case by simp
-next
-  case (Cons x xs)
-  from Cons have "\<And>y. y \<in> set (x # xs) \<Longrightarrow> f y = g y" by auto
-  then have "\<And>y. y \<in> set xs \<Longrightarrow> f y = g y" by auto
-  with Cons have "list f xs = list g xs" by auto
-  with Cons have "list f (x # xs) = list g (x # xs)" by auto
-  with Cons show "list f (x # xs) = list g ys" by auto
-qed
-
-lemma list_yield_cong [fundef_cong, recdef_cong]:
-  "\<lbrakk> \<And>x. x \<in> set xs \<Longrightarrow> f x = g x; xs = ys \<rbrakk>
-    \<Longrightarrow> list_yield f xs = list_yield g ys"
-proof (induct xs arbitrary: ys)
-  case Nil then show ?case by simp
-next
-  case (Cons x xs)
-  from Cons have "\<And>y. y \<in> set (x # xs) \<Longrightarrow> f y = g y" by auto
-  then have "\<And>y. y \<in> set xs \<Longrightarrow> f y = g y" by auto
-  with Cons have "list_yield f xs = list_yield g xs" by auto
-  with Cons have "list_yield f (x # xs) = list_yield g (x # xs)" by auto
-  with Cons show "list_yield f (x # xs) = list_yield g ys" by auto
-qed
 
 text {*
   For an example, see HOL/ex/Random.thy.
